src/GenHigh.v
@@ -1804,3 +1804,23 @@ Proof.
 Qed.
 
 
+Lemma bigcup_cons_setI_subset_compat_backtrack_weak
+      {A} (n : nat) (g g' : G (option A)) (l l' : seq (nat * G (option A))) :
+  (forall s, isSome :&: semGenSize g s  \subset isSome :&: semGenSize g' s) ->
+  (forall s, \bigcup_(x in (l :&: (fun x => x.1 <> 0))) (isSome :&: semGenSize x.2 s) \subset
+        \bigcup_(x in (l' :&: (fun x => x.1 <> 0))) (isSome :&: semGenSize x.2 s)) ->
+  (forall s, \bigcup_(x in (((n, g) :: l) :&: (fun x => x.1 <> 0))) (isSome :&: semGenSize x.2 s) \subset
+        \bigcup_(x in (((n, g') :: l') :&: (fun x => x.1 <> 0))) (isSome :&: semGenSize x.2 s)).
+Proof.
+  intros. eapply bigcup_cons_setI_subset_compat_backtrack; eauto.
+Qed.
+
+Lemma bigcup_cons_setI_subset_pres_backtrack_weak
+      {A} (n : nat) (g : G (option A)) (l l' : seq (nat * G (option A))) :
+  (forall s, \bigcup_(x in (l :&: (fun x => x.1 <> 0))) (isSome :&: semGenSize x.2 s) \subset
+        \bigcup_(x in (l' :&: (fun x => x.1 <> 0))) (isSome :&: semGenSize x.2 s)) ->
+  (forall s, \bigcup_(x in (l :&: (fun x => x.1 <> 0))) (isSome :&: semGenSize x.2 s) \subset
+         \bigcup_(x in ((n, g) :: l') :&: (fun x => x.1 <> 0)) (isSome :&: semGenSize x.2 s)).
+Proof.
+  intros. eapply bigcup_cons_setI_subset_pres_backtrack; eauto.
+Qed.
